\documentclass{article}
\usepackage[utf8]{inputenc}
\usepackage{amsmath}
\usepackage{environ}
\usepackage[T2A,T1]{fontenc}
\usepackage[russian]{babel}
\usepackage[letterpaper,top=2cm,bottom=2cm,left=3cm,right=3cm,marginparwidth=1.75cm]{geometry}

\begin{document}

\textbf{â„– 18} 
\large

$$ \lim\limits_{x \to \infty} \frac{\ln{\cos{\frac{\pi}{x}}}}{\tg{\frac{\pi}{x^2}}} 
= \frac{0}{0}
= \lim\limits_{x \to \infty} \frac{ (\frac{1}{\cos{\frac{\pi}{x}}}) (-\sin{\frac{\pi}{x}}) (-\frac{1}{x^2}) }{-\frac{2\pi}{x^3\cos^2{\frac{\pi}{x}}}} 
= -\frac{1}{2} \lim\limits_{x \to \infty} \frac{\tg{\frac{\pi}{x}} \ \cos^2{\frac{\pi}{x^2}}}{\frac{1}{x}}
= \frac{0}{0}
= $$  

$$ = -\frac{1}{2} \lim\limits_{x \to \infty} \frac{ \frac{1}{\cos^2{\frac{\pi}{x}}} (-\frac{\pi}{x^2}) (\cos^2{\frac{\pi}{x^2}}) + (\tg{\frac{\pi}{x}}) (2\cos{\frac{\pi}{x^2}}) (-\sin{\frac{\pi}{x^2}}) (-\frac{2\pi}{x^3}) }{-\frac{1}{x^2}} $$

$$ = -\frac{1}{2} \lim\limits_{x \to \infty} \left( \underbrace{\frac{\pi \cos^2{\frac{\pi}{x^2}} x^2}{x^2 \cos^2{\frac{\pi}{x}}}}_{\pi} - \underbrace{(\tg{\frac{\pi}{x}}) (\sin{\frac{2\pi}{x^2}}) (\frac{2\pi}{x})}_{0} \right) 
= -\frac{\pi}{2}$$

\end{document}