\documentclass{article}
\usepackage[utf8]{inputenc}
\usepackage{amsmath}
\usepackage[letterpaper,top=2cm,bottom=2cm,left=3cm,right=3cm,marginparwidth=1.75cm]{geometry}

\begin{document}

\textbf{â„– 14} 

\Large

$$ x_{n+1} = \left(1-\frac{1}{n+1}\right)x_n+\frac{1}{n+1} $$

$$ x_{1} = 2 $$

$$ x_{2} = \left(1-\frac{1}{2}\right)2+\frac{1}{2} 
= \frac{1}{2} $$

$$ x_{3} = \left(1-\frac{1}{3}\right)\frac{3}{2}+\frac{1}{3} 
= \frac{1}{2} + \frac{1}{3} 
= \frac{5}{6} $$

$$ x_{4} = \left(1-\frac{1}{4}\right)\frac{5}{6}+\frac{1}{4} 
= \frac{15}{24} + \frac{1}{4} 
= \frac{21}{24}
$$

$$ \Rightarrow \lim_{n\to\infty} x_n = 1 $$


\end{document}