\documentclass{article}
\usepackage[utf8]{inputenc}
\usepackage{amsmath}
\usepackage{environ}
\usepackage[T2A,T1]{fontenc}
\usepackage[russian]{babel}
\usepackage[letterpaper,top=2cm,bottom=2cm,left=3cm,right=3cm,marginparwidth=1.75cm]{geometry}
\usepackage{xcolor}

\begin{document}
\textbf{№ 21} 
\\
\\ см. также {\color{blue}MAF} 2018-03-03 olympiad № 20
\\ см. также {\color{red}MAE} 2021-04-24 olympiad № 21
\\ см. также {\color{red}MAE} 2021-07-31 exam № 12

$$ \sum_{n=1}^{\infty} \frac{1}{16n^2-8n-3} $$

\begin{enumerate}

\item Transform the denominator

$$ D = (-8)^2 + (-4)\times16\times(-3)=256=16^2 $$

$$ n_1 = \frac{8+16}{32}=\frac{24}{32} = \frac{3}{4} $$
$$ n_2 = \frac{8-16}{32}=-\frac{1}{4} $$

$$\sum_{n=1}^{\infty} \frac{1}{16n^2-8n-3} 
= \sum_{n=1}^{\infty} \frac{1}{16(n+\frac{1}{4})(n-\frac{3}{4})} 
= \sum_{n=1}^{\infty} \frac{1}{(4n+1)(4n-3)}$$

\item Divide the denominator

$$\frac{1}{(4n+1)(4n-3)} 
= \frac{A}{4n+1} + \frac{B}{4n-3} 
= \frac{A(4n-3)+B(4n+1)}{(4n+1)(4n-3)} 
= \frac{4An-3A+4Bn+B}{(4n+1)(4n-3)}$$

$$4An-3A+4Bn+B = 1$$

$$
\left\{
  \begin{array}{ccc}
    4A + 4B = 0 \\
    -3A+B = 1 \\
  \end{array}\Leftrightarrow
\right.
\left\{
  \begin{array}{ccc}
    A = -B \\
    4B = 1 \\
  \end{array}\Leftrightarrow
\right.
\left\{
  \begin{array}{ccc}
    A = =\frac{1}{4} \\
    B = \frac{1}{4} \\
  \end{array}
\right.
$$

$$ \sum_{n=1}^{\infty} \frac{1}{(4n+1)(4n-3)} = 
\sum_{n=1}^{\infty} \left(\frac{1}{4(4n-3)} - \frac{1}{4(4n+1)}\right) $$

\item Find the sum of the series

$$ \sum_{n=1}^{\infty} \left(\frac{1}{4(4n-3)} - \frac{1}{4(4n+1)}\right) 
= S_n = a_1+a_2+...+a_{n-1}+a_n = $$
$$ = \frac{1}{4} - \underbrace{\frac{1}{20} + \frac{1}{20}}_{0} - \underbrace{\frac{1}{36} + \frac{1}{36}}_{0} - \frac{1}{52} + ..... - \frac{1}{4(4n+1)} = \frac{1}{4} - \frac{1}{4(4n+1)}$$

\item Find the limit
$$S = \lim_{n\to\infty} S_n 
= \lim_{n\to\infty} \left(\frac{1}{4} - \underbrace{\frac{1}{4(4n+1)}}_{0}\right) 
= \frac{1}{4} $$


\end{enumerate}
\end{document}