\documentclass{article}
\usepackage[utf8]{inputenc}
\usepackage{amsmath}
\usepackage{environ}
\usepackage[T2A,T1]{fontenc}
\usepackage[russian]{babel}
\usepackage[letterpaper,top=2cm,bottom=2cm,left=3cm,right=3cm,marginparwidth=1.75cm]{geometry}
\usepackage{xcolor}

\begin{document}
\textbf{№ 22} 

$$ \int_{0}^{1} \frac{1}{x^2+3x+2} dx 
= \int_{0}^{1} \frac{1}{(x+1)(x+2)} dx  $$

\begin{enumerate}
\item Разбиваем подынтегральное выражение на части

$$\frac{1}{(x+1)(x+2)}
= \frac{A}{x+1} + \frac{B}{x+2} 
= \frac{A(x+2)+B(x+1)}{(x+1)(x+2)} 
= \frac{Ax+2A+Bx+B}{(x+1)(x+2)}$$

$$ Ax+2A+Bx+B = 1 $$

$$
\left\{
  \begin{array}{ccc}
    Ax+Bx = 0 \\
    2A+B = 1 \\
  \end{array}
\right  
    \Leftrightarrow
\left\{
  \begin{array}{ccc}
    A = -B \\
    -B = 1 \\
  \end{array}
\right
    \Leftrightarrow
\left\{
  \begin{array}{ccc}
    A = 1 \\
    B = -1 \\
  \end{array}
 \right.
$$

\item Решаем интегралs
$$ \int_{0}^{1} \frac{1}{(x+1)(x+2)} dx 
= \int_{0}^{1} \frac{1}{x+1} dx - \int_{0}^{1} \frac{1}{x+2} dx  
= \ln{(x+1)} \bigg\vert_{0}^{1} - \ln{(x+2)} \bigg\vert_{0}^{1}
= $$

$$ = (\ln{2} - 0) - (\ln{3} - \ln{2}) 
= 2\ln{2}-\ln{3} $$

\end{enumerate}
\end{document}