\documentclass{article}
\usepackage[utf8]{inputenc}
\usepackage{amsmath}
\usepackage{environ}
\usepackage[T2A,T1]{fontenc}
\usepackage[russian]{babel}
\usepackage{hyperref}
\usepackage[letterpaper,top=2cm,bottom=2cm,left=3cm,right=3cm,marginparwidth=1.75cm]{geometry}

\begin{document}

\textbf{№ 3} 
\\
\\ also look MAE 2021-06-26 olympiad № 2

\begingroup

\Large

$$ = \lim\limits_{x \to 0} \left( 1+\sh{x}-\sin{x} \right)^{\frac{1}{x^3}}
= 1^{\infty}
= \lim\limits_{x \to 0} \left( 1+\sh{x}-\sin{x} \right)^{\frac{1}{x^3}\frac{1}{\sh{x}-\sin{x}}\frac{\sh{x}-\sin{x}}{1}} $$

$$ = e^{\lim\limits_{x \to 0}\frac{\sh{x}-\sin{x}}{x^3}}
= \begin{Vmatrix} \sh{x} = \frac{e^x-e^{-x}}{2} \end{Vmatrix} 
= e^{\lim\limits_{x \to 0}\frac{\frac{1}{2}(e^x-e^{-x})-\sin{x}}{x^3}}
= e^{\frac{0}{0}} 
= $$

$$ = e^{\lim\limits_{x \to 0}\frac{\frac{1}{2}(e^x+e^{-x})-\cos{x}}{3x^2}}
= e^{\frac{0}{0}}
= e^{\lim\limits_{x \to 0}\frac{\frac{1}{2}(e^x-e^{-x})+\sin{x}}{6x}}
= e^{\frac{0}{0}}
= $$

$$ = e^{\lim\limits_{x \to 0}\frac{\frac{1}{2}(e^x+e^{-x})+\cos{x}}{6}}
= e^{\frac{1}{3}}
$$

\endgroup
\end{document}