\documentclass{article}
\usepackage[utf8]{inputenc}
\usepackage{amsmath}
\usepackage{environ}
\usepackage[T2A,T1]{fontenc}
\usepackage[russian]{babel}
\usepackage[letterpaper,top=2cm,bottom=2cm,left=3cm,right=3cm,marginparwidth=1.75cm]{geometry}

\begin{document}

\textbf{â„– 13} 
\large

$$ \lim\limits_{x \to \infty} x \left( \ln{(x+1)} - \ln{(x-1)} \right)
= \frac{0}{0}
= \lim\limits_{x \to \infty} \frac{\left( \ln{(x+1)} - \ln{(x-1)} \right)'}{\left( \frac{1}{x} \right)'}
= $$

$$ = \lim\limits_{x \to \infty} \frac{\frac{1}{x+1} - \frac{1}{x-1}}{-\frac{1}{x^2}}
= \lim\limits_{x \to \infty} \frac{\frac{-2}{(x+1)(x-1)}}{-\frac{1}{x^2}} 
= \lim\limits_{x \to \infty} \frac{2x^2}{(x+1)(x-1)}
= 2 \lim\limits_{x \to \infty} \frac{x^2}{x^2-1}
= $$

$$ 2 \lim\limits_{x \to \infty} \frac{1}{1- \frac{1}{x^2}}
= 2 $$

\end{document}