\documentclass{article}
\usepackage[utf8]{inputenc}
\usepackage{amsmath}
\usepackage{environ}
\usepackage[T2A,T1]{fontenc}
\usepackage[russian]{babel}
\usepackage[letterpaper,top=2cm,bottom=2cm,left=3cm,right=3cm,marginparwidth=1.75cm]{geometry}

\begin{document}

\textbf{â„– 2} 
\large

$$ \lim\limits_{x \to \infty} \left( \sqrt{x+3} - \sqrt{x-1} \right) \sqrt{x}
= \lim\limits_{x \to \infty} \frac{ \left( \sqrt{x+3} - \sqrt{x-1} \right)  \left( \sqrt{x+3} + \sqrt{x-1} \right) \sqrt{x}}{\left( \sqrt{x+3} + \sqrt{x-1} \right)}
= $$  

$$ = \lim\limits_{x \to \infty} \frac{ \left( x+3-x+1 \right) \sqrt{x}}{\sqrt{x+3} + \sqrt{x-1}} 
= 4\lim\limits_{x \to \infty} \frac{ \sqrt{x}}{\sqrt{x+3} + \sqrt{x-1}} 
= 4\lim\limits_{x \to \infty} \frac{1}{\sqrt{1+\frac{3}{x}} + \sqrt{1-\frac{1}{x}}} 
= 2 $$

\end{document}