\documentclass{article}
\usepackage[utf8]{inputenc}
\usepackage{amsmath}
\usepackage{environ}
\usepackage[T2A,T1]{fontenc}
\usepackage[russian]{babel}
\usepackage{hyperref}
\usepackage[letterpaper,top=2cm,bottom=2cm,left=3cm,right=3cm,marginparwidth=1.75cm]{geometry}

\begin{document}

\textbf{№ 14} 

\begingroup
\Large

$$ \lim\limits_{n\to \infty} \left( \frac{\sqrt[n]{a} + \sqrt[n]{b} + \sqrt[n]{c}}{3} \right)^{n}
= \lim\limits_{n\to \infty} \left( 1 + \frac{\sqrt[n]{a} + \sqrt[n]{b} + \sqrt[n]{c} - 3}{3} \right)^{n}
= 1^{\infty} $$

$$ = \lim\limits_{n\to \infty} \left( 1 + \frac{\sqrt[n]{a} + \sqrt[n]{b} + \sqrt[n]{c} - 3}{3} \right)^{n \times \frac{\sqrt[n]{a} + \sqrt[n]{b} + \sqrt[n]{c} - 3}{3} \times \frac{3}{\sqrt[n]{a} + \sqrt[n]{b} + \sqrt[n]{c} - 3}} 
= $$

$$ = e^{\lim\limits_{n\to \infty} \frac{\sqrt[n]{a} + \sqrt[n]{b} + \sqrt[n]{c} - 3}{\frac{3}{n}}}
$$

\begin{enumerate}
\item Решаем предел
$$ \lim\limits_{n\to \infty} \frac{\sqrt[n]{a} + \sqrt[n]{b} + \sqrt[n]{c} - 3}{\frac{3}{x}}
= \lim\limits_{n\to \infty} \frac{ -\frac{1}{n^2}\sqrt[n]{a}\ln{a} + -\frac{1}{n^2}\sqrt[n]{b}\ln{b} + -\frac{1}{n^2}\sqrt[n]{c}\ln{c} }{-\frac{3}{n^2}}$$

$$ \frac{\ln{a} + \ln{b} + \ln{c}}{3}
$$

\item Подставляем в степень e
$$ e^{\frac{\ln{a} + \ln{b} + \ln{c}}{3}}
= e^{\frac{\ln{abc}}{3}}
= e^{\ln{(abc)}^{\frac{1}{3}}}
= (abc)^{\frac{1}{3}}$$

\end{enumerate}
\endgroup
\end{document}