\documentclass{article}
\usepackage[utf8]{inputenc}
\usepackage{amsmath}
\usepackage{environ}
\usepackage[T2A,T1]{fontenc}
\usepackage[russian]{babel}
\usepackage{hyperref}
\usepackage[letterpaper,top=2cm,bottom=2cm,left=3cm,right=3cm,marginparwidth=1.75cm]{geometry}

\begin{document}

\textbf{â„– 16} 

\begingroup
\Large

$$ \lim\limits_{x\to 1} \left( 3x^{\frac{1}{3}} - 2x^{\frac{1}{2}} \right)^{\frac{1}{\ln{x}}}
= 1^{\infty}
= \lim\limits_{x\to 1} \left( 1 + (3x^{\frac{1}{3}} - 2x^{\frac{1}{2}} - 1) \right)^{\frac{1}{\ln{x}} \times \frac{1}{3x^{\frac{1}{3}} - 2x^{\frac{1}{2}} - 1} \times \frac{3x^{\frac{1}{3}} - 2x^{\frac{1}{2}} - 1}{1}}$$

$$ e^{\lim\limits_{x\to 1} \frac{3x^{\frac{1}{3}} - 2x^{\frac{1}{2}} - 1}{\ln{x}}}
= \frac{0}{0}
= e^{\lim\limits_{x\to 1} \frac{x^{-\frac{2}{3}} - x^{\frac{1}{2}}}{\frac{1}{x}}}
= e^{0}
= 1$$

\endgroup
\end{document}