\documentclass{article}
\usepackage[utf8]{inputenc}
\usepackage{amsmath}
\usepackage{environ}
\usepackage[T2A,T1]{fontenc}
\usepackage[russian]{babel}
\usepackage[letterpaper,top=2cm,bottom=2cm,left=3cm,right=3cm,marginparwidth=1.75cm]{geometry}
\usepackage{xcolor}

\begin{document}
\textbf{№ 3} 

\begin{enumerate}
\item Раскладываем интеграл
$$ \int_{1}^{2} \frac{x+3}{3x^2-x^3} dx $$

$$\frac{x+3}{3x^2-x^3}
=-\frac{x+3}{x^2(x-3)}
= \frac{A}{x} + \frac{B}{x^2} + \frac{C}{x-3} 
= \frac{x^2(A+C)+x(B-3A)-3B}{x^2(x-3)} $$

$$ x^2(A+C)+x(B-3A)-3B = x+3 $$

$$
\left\{
  \begin{array}{ccc}
    -3B = 3 \\
    B-3A = 1 \\
    C+A = 0
  \end{array}
\right.  
    \Leftrightarrow
\left\{
  \begin{array}{ccc}
    A = -\frac{2}{3} \\
    B = -1 \\
    C = \frac{2}{3}
  \end{array}
\right. 
$$

\item Решаем нтегралы
$$ -\int_{1}^{2} \left( -\frac{2}{3x} - \frac{1}{x^2} + \frac{2}{3(x-3)} \right) dx  
= \frac{2}{3}\int_{1}^{2} \frac{1}{x}dx + \int_{1}^{2}\frac{1}{x^2} - \frac{2}{3}\int_{1}^{2}\frac{1}{x-3} dx
= $$

$$ = \left( \frac{2}{3} \ln{\left| x \right|} - \frac{1}{x} - \frac{2}{3}\ln{\left| x-3 \right|} \right) \bigg\vert_{1}^{2}
= \left( \frac{2}{3} \ln{2} - \frac{1}{2} - \frac{2}{3}\ln{1} \right) - \left( \frac{2}{3} \ln{1} - \frac{1}{1} - \frac{2}{3}\ln{2} \right)
= \frac{4}{3} \ln{2} + \frac{1}{2} $$

\end{enumerate}
\end{document}