\documentclass{article}
\usepackage[utf8]{inputenc}
\usepackage{amsmath}
\usepackage{environ}
\usepackage[T2A,T1]{fontenc}
\usepackage[russian]{babel}
\usepackage{hyperref}
\usepackage[letterpaper,top=2cm,bottom=2cm,left=3cm,right=3cm,marginparwidth=1.75cm]{geometry}

\begin{document}

\textbf{â„– 4} 

\begingroup
\Large

$$ \lim\limits_{x\to 0} \frac{(x+\sqrt{1+x^2})^4 - (x-\sqrt{1+x^2})^4}{x}
= \frac{0}{0}
= $$

$$ = \lim\limits_{x\to 0} 4(x+\sqrt{1+x^2})^3 \left( 1+\frac{2x}{2\sqrt{1+x^2}} \right) - 4(x-\sqrt{1+x^2})^3 \left( 1-\frac{2x}{2\sqrt{1+x^2}} \right) $$

$$ = 4(1+0) - 4(-1)(1-0) 
= 8 
$$

\endgroup
\end{document}


