\documentclass{article}
\usepackage[utf8]{inputenc}
\usepackage{amsmath}
\usepackage{environ}
\usepackage[T2A,T1]{fontenc}
\usepackage[russian]{babel}
\usepackage{hyperref}
\usepackage[letterpaper,top=2cm,bottom=2cm,left=3cm,right=3cm,marginparwidth=1.75cm]{geometry}

\begin{document}

\textbf{№ 6} 

\begingroup
\Large

$$ \lim\limits_{n\to \infty} \left( -1 + \frac{1}{n} \right)^{n}
= \lim\limits_{n\to \infty} \left( 1 - \frac{2n+1}{n} \right)^{n}
= 1^{\infty}
= $$

$$ = \lim\limits_{n\to \infty} \left( 1 - \frac{2n+1}{n} \right)^{n (-\frac{n}{2n+1}) (=\frac{2n+1}{n})}
= \lim\limits_{n\to \infty} e^{-(2n+1)}$$

$\Rightarrow$ неопределенность (E)

\endgroup
\end{document}


