\documentclass{article}
\usepackage[utf8]{inputenc}
\usepackage{amsmath}
\usepackage{environ}
\usepackage[T2A,T1]{fontenc}
\usepackage[russian]{babel}
\usepackage[letterpaper,top=2cm,bottom=2cm,left=3cm,right=3cm,marginparwidth=1.75cm]{geometry}

\begin{document}
\textbf{â„– 2} 

$$ \lim\limits_{x \to e} \frac{e^x-x^e}{(x-e)^2} 
= \frac{0}{0} 
= \lim\limits_{x \to e} \frac{e^x - e \cdot x^{e-1}}{2x-2e}
= \frac{0}{0} 
= \lim\limits_{x \to e} \frac{e^x - e \cdot (e-1) \cdot x^{e-2}}{2} 
= \frac{e^e - (e^2-e) \cdot e^{e-2}}{2} 
= \frac{e^{e-1}}{2} $$

\end{document}