\documentclass{article}
\usepackage[utf8]{inputenc}
\usepackage{amsmath}
\usepackage{environ}
\usepackage[T2A,T1]{fontenc}
\usepackage[russian]{babel}
\usepackage[letterpaper,top=2cm,bottom=2cm,left=3cm,right=3cm,marginparwidth=1.75cm]{geometry}

\begin{document}

\textbf{â„– 23} 
\large

$$ \int_{0}^{1} x^2e^{-x} \ dx 
= \begin{Vmatrix} \int f \,dg = fg - \int g \ df \end{Vmatrix} =
  \begin{Vmatrix} f = x^2 &  g = -e^{-x} \\
                 df = 2x \ dx  & dg = e^{-x} \ dx \end{Vmatrix} 
= $$

$$ = -x^2e^{-x} + 2 \int x e^{-x} \ dx 
= \begin{Vmatrix} f = x &  g = -e^{-x} \\
                  df = dx  & dg = e^{-x} \ dx \end{Vmatrix}
= -x^2e^{-x} + 2 \left( -xe^{-x} + \int e^{-x} \ dx \right) 
= $$

$$ = \left( -x^2e^{-x} - 2  \left( xe^{-x} + e^{x} \right) \right) \bigg\vert_{0}^{1} 
= \left( -\frac{1}{e} - 2  \left(\frac{1}{e} + \frac{1}{e} \right) \right) - (-2) 
= -\frac{1}{e} - \frac{4}{e} + 2
= 2 - \frac{5}{e} $$

\end{document}