\documentclass{article}
\usepackage[utf8]{inputenc}
\usepackage{amsmath}
\usepackage{environ}
\usepackage[T2A,T1]{fontenc}
\usepackage[russian]{babel}
\usepackage[letterpaper,top=2cm,bottom=2cm,left=3cm,right=3cm,marginparwidth=1.75cm]{geometry}

\begin{document}

\textbf{â„– 7} 
\Large

$$ \lim\limits_{x \to 0} \left( \sqrt{1+x}-x \right)^{\frac{1}{x}}
= 1^{\infty}
= e^{\lim\limits_{x \to 0} \ln{\left( \sqrt{1+x}-x \right)^{\frac{1}{x}}}}
= e^{\lim\limits_{x \to 0} \frac{\ln{\left( \sqrt{1+x}-x \right)}}{x}} 
= \frac{0}{0}
= $$

$$ = e^{\lim\limits_{x \to 0} \frac{\frac{1}{\sqrt{1+x}-x} \cdot \left( \frac{1}{2\sqrt{1+x}}-1 \right)}{1}} 
= e^{\frac{\frac{1}{2}-1}{1}} 
= e^{-\frac{1}{2}} 
= \frac{1}{\sqrt{e}} $$

\end{document}