\documentclass{article}
\usepackage[utf8]{inputenc}
\usepackage{amsmath}
\usepackage{environ}
\usepackage[T2A,T1]{fontenc}
\usepackage[russian]{babel}
\usepackage[letterpaper,top=2cm,bottom=2cm,left=3cm,right=3cm,marginparwidth=1.75cm]{geometry}
\usepackage{xcolor}

\begin{document}
\textbf{â„– 19} 

$$ \lim\limits_{x\to \infty} \frac{1}{n} \sum_{k=3}^{n} \frac{3}{k^2-k-2}
= \lim\limits_{x\to \infty} \frac{1}{n} \sum_{k=3}^{n} \frac{3}{(k+1)(k-2)}
= \lim\limits_{x\to \infty} \frac{1}{n} \sum_{k=3}^{n} \left( \frac{1}{k-2} - \frac{1}{k+1} \right)
= $$

$$ = \lim\limits_{x\to \infty} \frac{1}{n} \left( 1+\frac{1}{2}+ ... + \frac{1}{n-2} \right) - \lim\limits_{x\to \infty} \frac{1}{n} \left( \frac{1}{4}+ ... + \frac{1}{n+1} \right)
= 0 - 0 
= 0 $$

\end{document}