\documentclass{article}
\usepackage[utf8]{inputenc}
\usepackage{amsmath}
\usepackage{environ}
\usepackage[T2A,T1]{fontenc}
\usepackage[russian]{babel}
\usepackage[letterpaper,top=2cm,bottom=2cm,left=3cm,right=3cm,marginparwidth=1.75cm]{geometry}
\usepackage{xcolor}

\begin{document}
\textbf{â„– 28} 

$$ f(x) = \int_{x}^{x^2} y\sqrt{1+y} \ dy, \ \ f'(2) = ? $$ 

$$ f(x)
= \int_{x}^{x^2} y\sqrt{1+y} \ dy
= \begin{vmatrix} z = 1+y \\
                 dz = dy \end{vmatrix}
= \int_{x}^{x^2} (z-1) \sqrt{z} dz
= \int_{x}^{x^2} \left( z^{\frac{3}{2}} - z^{\frac{1}{2}} \right)
= \left( \frac{2}{5} z^{\frac{5}{2}} - \frac{2}{3} z^{\frac{3}{2}} \right) \bigg\vert_{x}^{x^2} 
= $$

$$ = \left( \frac{2}{5} (1+y)^{\frac{5}{2}} - \frac{2}{3} (1+y)^{\frac{3}{2}} \right) \bigg\vert_{x}^{x^2} 
= \left( \frac{2}{5} (1+x^2)^{\frac{5}{2}} - \frac{2}{3} (1+x^2)^{\frac{3}{2}} \right) - \left( \frac{2}{5} (1+x)^{\frac{5}{2}} - \frac{2}{3} (1+x)^{\frac{3}{2}} \right) $$

$$ f'(x) 
= \left( \frac{2}{5} \cdot \frac{5}{2} \cdot (1+x^2)^{\frac{3}{2}} \cdot 2x - \frac{2}{3} \cdot \frac{3}{2} \cdot (1+x^2)^{\frac{3}{2} \cdot }2x \right) - \left( \frac{2}{5} \cdot \frac{5}{2} \cdot (1+x)^{\frac{5}{2}} - \frac{2}{3} \cdot \frac{3}{2} \cdot (1+x)^{\frac{3}{2}} \right) $$

$$ f'(2)
= \left( 4(1+4)^{\frac{3}{2}} - 4(1+4)^{\frac{3}{2}} \right) - \left( (1+2)^{\frac{5}{2}} - (1+2)^{\frac{3}{2}} \right) 
= 4\sqrt{5^3} - 4\sqrt{5} - \left( \sqrt{3^3} - \sqrt{3} \right) 
= 16\sqrt{5} - 2\sqrt{3} $$

\end{document}