\documentclass{article}
\usepackage[utf8]{inputenc}
\usepackage{amsmath}
\usepackage{environ}
\usepackage[T2A,T1]{fontenc}
\usepackage[russian]{babel}
\usepackage[letterpaper,top=2cm,bottom=2cm,left=3cm,right=3cm,marginparwidth=1.75cm]{geometry}
\usepackage{xcolor}

\begin{document}
\textbf{№ 33}
\Large

$$ \lim\limits_{x\to 0} \frac{(1-\sin{x})^{\ln{(x^2+1)}}-1}{x^3} $$

\begin{enumerate}
\item Упрощаем $\ln{(x^2+1)}$
$$ \lim\limits_{x\to 0} \ln{(x^2+1)} 
= \lim\limits_{x\to 0} \ln{(x^2+1)^{x^2 \cdot \frac{1}{x^2}}} 
= \ln{e^{x^2}}
= x^2 $$

\item Упрощаем $ (1-\sin{x})^{\ln{(x^2+1)}} $
$$ \lim\limits_{x\to 0} (1-\sin{x})^{\ln{(x^2+1)}} 
= \lim\limits_{x\to 0} (1-\sin{x})^{x^2} 
= \lim\limits_{x\to 0} (1-\sin{x})^{x^2} 
= e^{-x^2\sin{x}} $$

\item Объединяем
$$ \lim\limits_{x\to 0} \frac{(1-\sin{x})^{\ln{(x^2+1)}}-1}{x^3} 
= \lim\limits_{x\to 0} \frac{e^{-x^2\sin{x}}-1}{x^3} 
= \lim\limits_{x\to 0} \frac{\frac{1}{e^{\frac{x^3\sin{x}}{x}}}-1}{x^3} 
= $$

$$ = \lim\limits_{x\to 0} \frac{\frac{1}{e^{x^3}}-1}{x^3}
= \lim\limits_{x\to 0} \frac{1-e^{x^3}}{x^3e^{x^3}}
= \lim\limits_{x\to 0} \frac{1-e^{x^3}}{x^3}
= \begin{vmatrix} x \to 0 \\
                  \lim\limits_{x\to 0} \frac{a^x-1}{x} = \ln{a} \end{vmatrix}
= -\ln{e}
= -1 $$

\end{enumerate}
\end{document}