\documentclass{article}
\usepackage[utf8]{inputenc}
\usepackage{amsmath}
\usepackage{environ}
\usepackage[T2A,T1]{fontenc}
\usepackage[russian]{babel}
\usepackage[letterpaper,top=2cm,bottom=2cm,left=3cm,right=3cm,marginparwidth=1.75cm]{geometry}
\usepackage{xcolor}

\begin{document}
\textbf{№ 12} 
\\
\\ см. также {\color{blue}MAF} 2018-03-03 olympiad № 20
\\ см. также {\color{red}MAE} 2021-04-24 olympiad № 21
\\ см. также {\color{red}MAE} 2021-07-31 exam № 12

$$\sum_{n=1}^{\infty} \frac{1}{25n^2-5n-6}$$

\begin{enumerate}

\item Transform the denominator

$$D = (-5)^2 + (-4)\times25\times(-6)=625=25^2$$

$$n_1 = \frac{5+25}{50}=\frac{3}{5}$$
$$n_2 = \frac{5-25}{50}=-\frac{2}{5}$$

$$\sum_{n=1}^{\infty} \frac{1}{25n^2-5n-6} = \sum_{n=1}^{\infty} \frac{1}{25(n+\frac{2}{5})(n-\frac{3}{5})} = \sum_{n=1}^{\infty} \frac{1}{(5n+2)(5n-3)}$$

\item Divide the denominator

$$\frac{1}{(5n+2)(5n-3)} = \frac{A}{5n+2} + \frac{B}{5n-3} 
= \frac{A(5n-3)+B(5n+2)}{(5n+2)(5n-3)} 
= \frac{5An-3A+5Bn+2B}{(5n+2)(5n-3)}$$

$$5An-3A+5Bn+2B = 1$$

$$
\left\{
  \begin{array}{ccc}
    5A + 5B = 0 \\
    -3A+2B = 1 \\
  \end{array}\Leftrightarrow
\right.
\left\{
  \begin{array}{ccc}
    A = -B \\
    5B = 1 \\
  \end{array}\Leftrightarrow
\right.
\left\{
  \begin{array}{ccc}
    A = =\frac{1}{5} \\
    B = \frac{1}{5} \\
  \end{array}
\right.
$$

$$ \sum_{n=1}^{\infty} \frac{1}{(5n+2)(5n-3)} = 
\sum_{n=1}^{\infty} \left(\frac{1}{5(5n-3)} - \frac{1}{5(5n+2)}\right) $$

\item Find the sum of the series

$$ \sum_{n=1}^{\infty} \left(\frac{1}{5(5n-3)} - \frac{1}{5(5n+2)}\right) 
= S_n = a_1+a_2+...+a_{n-1}+a_n = $$
$$ = \frac{1}{10} - \underbrace{\frac{1}{35} + \frac{1}{35}}_{0} - \underbrace{\frac{1}{60} + \frac{1}{60}}_{0} - \frac{1}{85} + ..... - \frac{1}{5(5n+2)} = \frac{1}{10} - \frac{1}{5(5n+2)}$$

\item Find the limit
$$S = \lim_{n\to\infty} S_n 
= \lim_{n\to\infty} \left(\frac{1}{10} - \underbrace{\frac{1}{5(5n+2)}}_{0}\right) 
= \frac{1}{10} $$


\end{enumerate}
\end{document}