\documentclass{article}
\usepackage[utf8]{inputenc}
\usepackage{amsmath}
\usepackage{environ}
\usepackage[T2A,T1]{fontenc}
\usepackage[russian]{babel}
\usepackage[letterpaper,top=2cm,bottom=2cm,left=3cm,right=3cm,marginparwidth=1.75cm]{geometry}
\usepackage{xcolor}

\begin{document}
\textbf{№ 17} 
\\
\\ смотри также {\color{red}MAE} 2017-07-31 exam № 14
\\ смотри также {\color{red}MAE} 2019-07-31 exam № 4
\\ смотри также {\color{red}MAE} 2021-07-31 exam № 17

\begingroup
$$ \lim_{n\to \infty} \left( \sqrt[3]{(n+a_1)(n+a_2)(n+a_3)} - n \right) 
= $$

\begin{enumerate}
\item Первое решение задачи

$$ \begin{Vmatrix} n=\frac{1}{z}, z=\frac{1}{n}, n\to \infty \ \Rightarrow z\to\frac{1}{\infty}=0 \end{Vmatrix} $$

$$ \lim_{z\to 0} \left(\frac{\sqrt[3]{(a_1z+1)(a_2z+1)(a_3z+1)} - 1}{z} \right) 
= \frac{0}{0}
= $$

$$ = \lim_{z\to 0} \left( \frac{a_1\sqrt[3]{(a_2z+1)(a_3z+1)}}{3\sqrt[3]{(a_1z+1)}} 
+ \frac{a_2\sqrt[3]{(a_1z+1)(a_3z+1)}}{3\sqrt[3]{(a_2z+1)}} 
+ \frac{a_3\sqrt[3]{(a_1z+1)(a_2z+1)}}{3\sqrt[3]{(a_3z+1)}} \right)
= $$

$$ = \frac{a_1+a_2+a_3}{3} $$

\item Второе решение задачи

\end{enumerate}
\endgroup
\end{document}