\documentclass{article}
\usepackage[utf8]{inputenc}
\usepackage{amsmath}
\usepackage{environ}
\usepackage[T2A,T1]{fontenc}
\usepackage[russian]{babel}
\usepackage{hyperref}
\usepackage[letterpaper,top=2cm,bottom=2cm,left=3cm,right=3cm,marginparwidth=1.75cm]{geometry}

\begin{document}

\textbf{â„– 9} 

\begingroup
\Large

$$ \lim\limits_{x \to +\infty} \left( x\ln{(x+e^x)} - x^2 \right)
= \lim\limits_{x \to +\infty} \left( x\ln{(e^x(1+\frac{x}{e^x}))} - x^2 \right)
= $$

$$ = \lim\limits_{x \to +\infty} \left( x^2 \ln{(1+\frac{x}{e^x})}^{\frac{e^x}{x}\frac{x}{e^x}} - x^2 \right)
= \lim\limits_{x \to +\infty} x^2 \left( e^{\frac{x}{e^x}} - 1 \right)
= x^2 - x^2 
= 0 $$

\endgroup
\end{document}