\documentclass{article}
\usepackage[utf8]{inputenc}
\usepackage{amsmath}
\usepackage{environ}
\usepackage[T2A,T1]{fontenc}
\usepackage[russian]{babel}
\usepackage{hyperref}
\usepackage[letterpaper,top=2cm,bottom=2cm,left=3cm,right=3cm,marginparwidth=1.75cm]{geometry}

\begin{document}

\textbf{â„– 17} 

\begingroup

$$ \lim\limits_{x\to +\infty} \left( \sqrt{x^4+x^2\sqrt{x^4+1}} - \sqrt{2x^4} \right)
=  \lim\limits_{x\to +\infty} \left( \frac{(\sqrt{x^4+x^2\sqrt{x^4+1}} - \sqrt{2x^4})(\sqrt{x^4+x^2\sqrt{x^4+1}} + \sqrt{2x^4})}{\sqrt{x^4+x^2\sqrt{x^4+1}} + \sqrt{2x^4}} \right)
= $$

$$ \lim\limits_{x\to +\infty} \frac{x^4+x^2\sqrt{x^4+1} - 2x^4}{\sqrt{x^4+x^2\sqrt{x^4+1}} + \sqrt{2x^4}}
= \lim\limits_{x\to +\infty} \frac{x^2\sqrt{x^4+1} - x^4}{\sqrt{x^4+x^2\sqrt{x^4+1}} + \sqrt{2x^4}}
= $$

$$ = \lim\limits_{x\to +\infty} \frac{(x^2\sqrt{x^4+1} - x^4)(x^2\sqrt{x^4+1} + x^4)}{(\sqrt{x^4+x^2\sqrt{x^4+1}} + \sqrt{2x^4})(x^2\sqrt{x^4+1} + x^4)} 
= \lim\limits_{x\to +\infty} \frac{x^4}{(\sqrt{x^4+x^2\sqrt{x^4+1}} + \sqrt{2x^4})(x^2\sqrt{x^4+1} + x^4)}
= $$

$$ = \lim\limits_{x\to +\infty} \frac{1}{(\sqrt{x^4+x^2\sqrt{x^4+1}} + \sqrt{2x^4})(\frac{\sqrt{x^4+1}}{x^2} + 1)}
= \frac{1}{\infty}
= 0 $$

\endgroup
\end{document}