\documentclass{article}
\usepackage[utf8]{inputenc}
\usepackage{amsmath}
\usepackage{environ}
\usepackage[T2A,T1]{fontenc}
\usepackage[russian]{babel}
\usepackage{hyperref}
\usepackage[letterpaper,top=2cm,bottom=2cm,left=3cm,right=3cm,marginparwidth=1.75cm]{geometry}

\begin{document}

\textbf{â„– 2} 

\begingroup
\Large

$$ \lim_{x\to 1} \left( \frac{2x+1}{x+2} \right)^{\frac{1}{x^2-3x+2}}
= \lim_{x\to 1} \left( \frac{2x+1}{x+2} \right)^{\frac{1}{(x-2)(x-1)}}
= 1^{\infty} 
= $$

$$ = e^{\lim\limits_{x\to 1} \ln{\left( \frac{2x+1}{x+2} \right)^{\frac{1}{(x-2)(x-1)}}}}
= e^{\lim\limits_{x\to 1} \frac{\ln{\left( \frac{2x+1}{x+2} \right)}}{(x-2)(x-1)}}
= e^{\frac{0}{0}}
= $$

$$ = e^{\lim\limits_{x\to 1} \frac{ \frac{x+2}{2x+1} \frac{(2(x+2) - 1(2x+1))}{(x+2)^2} }{2x-3} }
= e^{\lim\limits_{x\to 1} \frac{ \frac{(2x+4-2x-1}{(x+2)(2x+1)} }{2x-3} } 
= e^{\lim\limits_{x\to 1} \frac{3}{(2x-3)(x+2)(2x+1)}} 
= $$

$$ = e^{\frac{3}{3\cdot3\cdot(-1)}}
= e^{-\frac{1}{3}}$$

\endgroup
\end{document}