\documentclass{article}
\usepackage[utf8]{inputenc}
\usepackage{amsmath}
\usepackage{environ}
\usepackage[T2A,T1]{fontenc}
\usepackage[russian]{babel}
\usepackage{hyperref}
\usepackage[letterpaper,top=2cm,bottom=2cm,left=3cm,right=3cm,marginparwidth=1.75cm]{geometry}

\begin{document}

\textbf{â„– 17} 

\begingroup
\Large

$$ \lim\limits_{x \to 0} \frac{e^x-\sqrt{2x+1}}{e^x-x-1}
= \frac{0}{0}
= \lim\limits_{x \to 0} \frac{e^x-\frac{2}{2\sqrt{2x+1}}}{e^x-1}
= \frac{0}{0} 
= \lim\limits_{x \to 0} \frac{e^x+\frac{1}{(2x+1)\sqrt{2x+1}}}{e^x} 
= 2 $$

\endgroup
\end{document}