\documentclass{article}
\usepackage[utf8]{inputenc}
\usepackage{amsmath}
\usepackage{environ}
\usepackage[T2A,T1]{fontenc}
\usepackage[russian]{babel}
\usepackage{hyperref}
\usepackage[letterpaper,top=2cm,bottom=2cm,left=3cm,right=3cm,marginparwidth=1.75cm]{geometry}

\begin{document}

\textbf{â„– 2} 

\begingroup
\Large

$$ \lim\limits_{x \to \infty} x\left( x+1-\sqrt{x^2+2x} \right)
= \lim\limits_{x \to \infty} \frac{x\left( x+1-\sqrt{x^2+2x} \right) \left( x+1+\sqrt{x^2+2x} \right)}{\left( x+1+\sqrt{x^2+2x} \right)}
= $$

$$ = \lim\limits_{x \to \infty} \frac{x\left( (x+1)^2-(x^2+2x) \right)}{x+1+\sqrt{x^2+2x}} 
= \lim\limits_{x \to \infty} \frac{x\left( x^2+2x+1-x^2-2x \right)}{x\left(1+\frac{1}{x}+\sqrt{1+\frac{2}{x}}\right)} 
= \frac{1}{2} $$

\endgroup
\end{document}