\documentclass{article}
\usepackage[utf8]{inputenc}
\usepackage{amsmath}
\usepackage{environ}
\usepackage[T2A,T1]{fontenc}
\usepackage[russian]{babel}
\usepackage{hyperref}
\usepackage[letterpaper,top=2cm,bottom=2cm,left=3cm,right=3cm,marginparwidth=1.75cm]{geometry}

\begin{document}

\textbf{â„– 1}
\Large

$$ \lim\limits_{x\to +\infty} x^2 \left( e^{\frac{1}{x}} - e^{\frac{1}{x+1}} \right) 
= \begin{vmatrix} \lim\limits_{z\to 0} \frac{a^{z} - 1}{z} = \ln{a} \end{vmatrix}
= \lim\limits_{x\to +\infty} x^2 \left( (e^{\frac{1}{x}} - 1) +  (e^{\frac{1}{x+1}} - 1) \right) 
= $$

$$ = \lim\limits_{x\to +\infty} \left( x \ \frac{e^{\frac{1}{x}} - 1}{\frac{1}{x}} - \frac{x^2}{x+1} \frac{ e^{\frac{1}{x+1}} -1 }{ \frac{1}{x+1} } \right)
= \lim\limits_{x\to +\infty} \left( x - \frac{x^2}{x+1} \right) 
= \lim\limits_{x\to +\infty} \frac{x}{x+1}
= 1$$

\end{document}