\documentclass{article}
\usepackage[utf8]{inputenc}
\usepackage{amsmath}
\usepackage{environ}
\usepackage[T2A,T1]{fontenc}
\usepackage[russian]{babel}
\usepackage[letterpaper,top=2cm,bottom=2cm,left=3cm,right=3cm,marginparwidth=1.75cm]{geometry}

\begin{document}

\textbf{â„– 11} 
\large

$$ \int_{-1}^{2} (2x+1)e^{-x} \ dx $$

$$ \begin{Vmatrix} \int f \,dg = fg - \int g \ df \end{Vmatrix} =
   \begin{Vmatrix} f = 2x+1 &  g = -e^{-x} \\
                  df = 2dx  & dg = e^{-x} \ dx \end{Vmatrix} $$

$$  \int_{-1}^{2} (2x+1)e^{-x} \ dx
= -(2x+1)e^{-x} + 2\int e^{-x} dx 
= \left( -(2x+1)e^{-x} - 2e^{-x} \right) \bigg\vert_{-1}^{2}
= $$

$$ = \left( -5e^{-2} - 2e^{-2} \right) - \left( e - 2e \right)
= e - \frac{7}{e^2}$$

\end{document}