\documentclass{article}
\usepackage[utf8]{inputenc}
\usepackage{amsmath}
\usepackage{environ}
\usepackage[T2A,T1]{fontenc}
\usepackage[russian]{babel}
\usepackage{hyperref}
\usepackage[letterpaper,top=2cm,bottom=2cm,left=3cm,right=3cm,marginparwidth=1.75cm]{geometry}

\begin{document}
\textbf{â„– 25}

$$ \lim\limits_{x\to +\infty} \left( \sqrt{x+2\sqrt{x}} - \sqrt{x} \right) 
= \lim\limits_{x\to +\infty} \frac{\left( \sqrt{x+2\sqrt{x}} - \sqrt{x} \right) \left( \sqrt{x+2\sqrt{x}} + \sqrt{x} \right) }{\left( \sqrt{x+2\sqrt{x}} + \sqrt{x} \right) } 
= \lim\limits_{x\to +\infty} \frac{x+2\sqrt{x} - x}{\sqrt{x+2\sqrt{x}} + \sqrt{x}}
= $$

$$ = \lim\limits_{x\to +\infty} \frac{2}{\sqrt{1+\frac{2\sqrt{x}}{x}} + 1} 
= \frac{2}{\sqrt{1} + 1} 
= 1 $$

\end{document}