\documentclass{article}
\usepackage[utf8]{inputenc}
\usepackage{amsmath}
\usepackage{environ}
\usepackage[T2A,T1]{fontenc}
\usepackage[russian]{babel}
\usepackage[letterpaper,top=2cm,bottom=2cm,left=3cm,right=3cm,marginparwidth=1.75cm]{geometry}

\begin{document}

\textbf{â„– 12} 

$$ \lim\limits_{x \to \infty} \left( \sqrt{x^4+x^2+x+1} - \sqrt{x^4+1} \right)
= \lim\limits_{x \to \infty} \frac{\left( \sqrt{x^4+x^2+x+1} - \sqrt{x^4+1} \right) \left( \sqrt{x^4+x^2+x+1} + \sqrt{x^4+1} \right)}{\left( \sqrt{x^4+x^2+x+1} + \sqrt{x^4+1} \right)}
= $$

$$ = \lim\limits_{x \to \infty} \frac{x^4+x^2+x+1-x^4-1}{\sqrt{x^4(1+\frac{1}{x^2}+\frac{1}{x^3}+\frac{1}{x^4})} + \sqrt{x^4(1+\frac{1}{x^4})}} 
= \lim\limits_{x \to \infty} \frac{x^2(1+\frac{1}{x})}{x^2\sqrt{1+\frac{1}{x^2}+\frac{1}{x^3}+\frac{1}{x^4}} + \sqrt{1+\frac{1}{x^4}}} 
= \frac{1}{2} $$

\end{document}