\documentclass{article}
\usepackage[utf8]{inputenc}
\usepackage{amsmath}
\usepackage{environ}
\usepackage[T2A,T1]{fontenc}
\usepackage[russian]{babel}
\usepackage{hyperref}
\usepackage[letterpaper,top=2cm,bottom=2cm,left=3cm,right=3cm,marginparwidth=1.75cm]{geometry}

\begin{document}

\textbf{â„– 10} 

\begingroup

\Large

$$ \int \frac{2x+3}{e^x} \,dx $$

$$ \begin{Vmatrix} \int f \,dg = fg - \int g \ df \end{Vmatrix} =
   \begin{Vmatrix} f = 2x+3 &  g = -e^{-x} \\
                  df = 2dx  & dg = \int dg = \int e^{-x} dx \end{Vmatrix} = $$

$$ = \int \frac{2x+3}{e^x} \,dx = -(2x+3)e^{-x} - \int -2 e^{-x}dx = $$

$$ = \begin{vmatrix} u = -x \\ 
                    du = -dx \\
                    dx = - du \end{vmatrix} 
= -e^{-x}(2x+3) -2 \int e^{u}du 
= -e^{-x}(2x+3) -2e^{-x}
= $$

$$ = e^{-x}(-(2x+3)-2)
= -\frac{2x+5}{e^{x}} $$

\endgroup
\end{document}