\documentclass{article}
\usepackage[utf8]{inputenc}
\usepackage{amsmath}
\usepackage{environ}
\usepackage[T2A,T1]{fontenc}
\usepackage[russian]{babel}
\usepackage[letterpaper,top=2cm,bottom=2cm,left=3cm,right=3cm,marginparwidth=1.75cm]{geometry}

\begin{document}

\textbf{№ 11} 


$$ \int \frac{13-6x}{6+x-x^2} dx 
= \int \frac{6x-13}{x^2-x-6} dx
= \int \frac{3(2x-1) - 10}{x^2-x-6} dx
= $$

$$ = 3 \int \frac{2x-1}{x^2-x-6} dx - 10 \int \frac{1}{x^2-x-6}dx
= 3 \int \frac{2x-1}{x^2-x-6} dx - 10 \int \frac{1}{(x+2)(x-3)}dx $$

\begin{enumerate}

\item Решаем первый интеграл
$$ 3 \int \frac{2x-1}{x^2-x-6} dx
= \begin{vmatrix}   u = x^2 - x - 6 \\ 
                    du = (2x-1)dx \end{vmatrix} 
= 3 \int \frac{1}{u}du 
= 3 \ln{\left| u \right|}
= 3 \ln{\left| x^2 - x - 6 \right|}
= 3 \ln{\left| (x-2)(x+3) \right|}$$

\item Решаем второй интеграл
$$ -10 \int \frac{1}{(x+2)(x-3)}dx $$

$$\frac{1}{(x+2)(x-3)} 
= \frac{A}{x+2} + \frac{B}{x-3} 
= \frac{A(x-3)+B(x+2)}{(x+2)(x-3)} 
= \frac{Ax-3A+Bx+2B}{(x+2)(x-3)}$$

$$Ax-3A+Bx+2B = 1$$

$$
\left\{
  \begin{array}{ccc}
    A + B = 0 \\
    -3A + 2B = 1 \\
  \end{array}
\right  
    \Leftrightarrow
\left\{
  \begin{array}{ccc}
    A = -B \\
    -5A = 1 \\
  \end{array}
\right
    \Leftrightarrow
\left\{
  \begin{array}{ccc}
    A = -\frac{1}{5} \\
    B = \frac{1}{5} \\
  \end{array}
 \right.
$$

$$ -10 \int \frac{1}{(x+2)(x-3)}dx 
= -10 \left( \int -\frac{1}{5(x+2)}dx + \int \frac{1}{5(x-3)}dx\right) 
= 2 \left( \int \frac{1}{x+2}dx - \int \frac{1}{x-3}dx \right)
= $$

$$ = 2 \left( \ln{\left| x+2 \right|} - \ln{\left| x-3 \right|} \right) $$

\item Складываем решение двух интегралов
$$ 3 \ln{\left| (x+2)(x-3) \right|} + 2 \left( \ln{\left| x+2 \right|} - \ln{\left| x-3 \right|} \right)
= \ln{\left| (x+2)^3 (x-3)^3 \right|} +  \ln{\left| x-3 \right|^{-2}} + \ln{\left| x+2 \right|^{2}} 
= $$

$$ = \ln{\left| (x+2)^5 (x-3) \right|}
= 5\ln{\left| x+2 \right|} + \ln{\left| x-3 \right|}$$

\end{enumerate}
\end{document}