\documentclass{article}
\usepackage[utf8]{inputenc}
\usepackage{amsmath}
\usepackage{environ}
\usepackage[T2A,T1]{fontenc}
\usepackage[russian]{babel}
\usepackage[letterpaper,top=2cm,bottom=2cm,left=3cm,right=3cm,marginparwidth=1.75cm]{geometry}

\begin{document}

\textbf{№ 16} 

$$ \int_{-\frac{\pi}{4}}^{\frac{\pi}{4}} \frac{\tg^3{x}+\cos{x}\sin{x}}{1+\tg^2{x}}dx 
= $$

Формула: $ 1+\tg^2{x} = \frac{1}{\cos^2{x}}$

$$ = \int_{-\frac{\pi}{4}}^{\frac{\pi}{4}} \frac{\sin^3{x}+\cos^4{x}\sin{x}}{\cos{x}}dx
= \int_{-\frac{\pi}{4}}^{\frac{\pi}{4}} \frac{\sin{x}(\sin^2{x} + \cos^4{x})}{\cos{x}}dx 
= \int_{-\frac{\pi}{4}}^{\frac{\pi}{4}} \frac{\sin{x}(\cos^4{x} - \cos^2{x} + 1)}{\cos{x}}dx
= $$


$$ = \begin{vmatrix}    u  = \cos{x} \\ 
                        du = \sin{x} dx \end{vmatrix}
=  -\int \frac{u^4-u^2+1}{u} \ du
= -\int u^3 \ du + \int u \ du - \int \frac{1}{u} \ du
= $$

$$ = -\frac{u^4}{4} + \frac{u^2}{2} - \ln{u}
= \left( -\frac{\cos^4{x}}{4} + \frac{\cos^2{x}}{2} - \ln{\cos{x}} \right) \bigg\vert_{-\frac{\pi}{4}}^{\frac{\pi}{4}}
= $$

так как функция $\cos{x}$ четная $f(-x) = f(x)$, то все это равно нулю

$$ = \left( -\frac{(\frac{\sqrt{2}}{2})^4}{4} + \frac{(\frac{\sqrt{2}}{2})^2}{2} - \ln{\frac{\sqrt{2}}{2}} \right) - \left( -\frac{(\frac{\sqrt{2}}{2})^4}{4} + \frac{(\frac{\sqrt{2}}{2})^2}{2} - \ln{\frac{\sqrt{2}}{2}} \right)
= 0$$



\end{document}