\documentclass{article}
\usepackage[utf8]{inputenc}
\usepackage{amsmath}
\usepackage[letterpaper,top=2cm,bottom=2cm,left=3cm,right=3cm,marginparwidth=1.75cm]{geometry}

\begin{document}

\textbf{â„– 18}

$$ \lim_{x\to 0} \left( \frac{\ln(e^x-x-1)}{\ln(x)} \right) 
= \frac{\infty}{\infty} 
= \lim_{x\to 0} \left( \frac{\frac{e^x-1}{e^x-x-1}}{\frac{1}{x}} \right)
= \lim_{x\to 0} \left( \frac{x(e^x-1)}{e^x-x-1} \right) 
= \frac{0}{0} = $$

$$ = \lim_{x\to 0} \left( \frac{e^x+xe^x-1}{e^x-1} \right)
= \frac{0}{0}
= \lim_{x\to 0} \left( \frac{e^x+xe^x+e^x}{e^x} \right)
= \frac{1+1}{1}
= 2 $$

\end{document}