\documentclass{article}
\usepackage[utf8]{inputenc}
\usepackage{amsmath}
\usepackage[letterpaper,top=2cm,bottom=2cm,left=3cm,right=3cm,marginparwidth=1.75cm]{geometry}

\begin{document}

\textbf{â„– 7}

\begin{enumerate}

\item First way to solve

$$ \lim_{x\to 0} \left( \frac{\ln(1-x^2)-2cosx+2}{1-e^{x^2}+xsinx} \right) 
= \frac{0}{0} 
= \lim_{x\to 0} \left( \frac{-\frac{2x}{1-x^2}+2sinx}{-2xe^{x^2}+sinx+xcosx} \right)
= \frac{0}{0} 
= $$

$$ = \lim_{x\to 0} \frac{\frac{-2(1-x^2)+2x(-2x)}{(1-x^2)^2}+2cosx}{-2e^{x^2}-4x^2e^{x^2}+2cosx-xsinx} 
= \lim_{x\to 0} \frac{-\frac{2(x^2+1)}{(1-x^2)^2}+2cosx}{-2e^{x^2}-4x^2e^{x^2}+2cosx-xsinx} 
= \frac{0}{0} 
= $$

$$ = \lim_{x\to 0} \frac{-2 \left( \frac{2x(1-x^2)^2-(x^2+1)(4x^3-4x)} {(1-x^2)^4}\right)-2sinx}{-2sinx-sinx-xcosx-4xe^{x^2}-8xe^{x^2}-8x^3e^{x^2}} 
= $$

$$ = \lim_{x\to 0} \frac{-2 \left( \frac{-2x^5-4x^3+6x} {(1-x^2)^4}\right)-2sinx}{-2sinx-sinx-xcosx-4xe^{x^2}-8xe^{x^2}-8x^3e^{x^2}}
= \frac{0}{0} 
= $$

$$ = \lim_{x\to 0} \frac{-2 \left( \frac{(-10x-12x^2+6)(1-x^2)^4-(-2x^5-4x^3+6x)(... + 1)} {(1-x^2)^8}\right)-2cosx}{-2cosx-cosx+xsinx-cosx-4e^{x^2}-8x^2e^{x^2}-8e^{x^2}-16x^2e^{x^2}-24x^2e^{x^2}-16x^4e^{x^2}}
= $$

$$ = \frac{-2-2\left( \frac{6-0}{1}\right)}{-2-1-1-4-8} 
= \frac{14}{16}
= \frac{7}{8}
$$

\item Second way to solve

Taylor series: $\sin{x}, \ \cos{x}, \ \ln{(1+x)}$ 

\end{enumerate}
\end{document}