\documentclass{article}
\usepackage[utf8]{inputenc}
\usepackage{amsmath}
\usepackage{environ}
\usepackage[T2A,T1]{fontenc}
\usepackage[russian]{babel}
\usepackage{hyperref}
\usepackage[letterpaper,top=2cm,bottom=2cm,left=3cm,right=3cm,marginparwidth=1.75cm]{geometry}

\begin{document}

\textbf{â„– 8} 

\begingroup
\Large

$$ ((\tg{x})^{x})'
= \left( e^{\ln{(\tg{x})^{x}}} \right)'
= \left( e^{x \ln{(\tg{x})}} \right)'
= e^{x \ln{(\tg{x})}} \left( x \ln{(\tg{x})} \right)'
= $$

$$ = e^{x \ln{(\tg{x})}} \left( \ln{(\tg{x})} + x \times \frac{1}{\tg{x}} \times \frac{1}{\cos^2{x}} \right)
= (\tg{x})^{x} \left( \ln{(\tg{x})} + \frac{x}{\tg{x} \cos^2{x}}\right)
= $$

$$ = \frac{(\tg{x})^{x}}{\tg{x}} \left( \tg{x}\ln{(\tg{x})} + \frac{x}{\cos^2{x}}\right)
= (\tg{x})^{x-1} \left( \tg{x}\ln{(\tg{x})} + \frac{x}{\cos^2{x}}\right)$$

\endgroup
\end{document}


