\documentclass{article}
\usepackage[utf8]{inputenc}
\usepackage{amsmath}
\usepackage{environ}
\usepackage[T2A,T1]{fontenc}
\usepackage[russian]{babel}
\usepackage{hyperref}
\usepackage[letterpaper,top=2cm,bottom=2cm,left=3cm,right=3cm,marginparwidth=1.75cm]{geometry}

\begin{document}

\textbf{â„– 14} 

\begingroup
\Large

$$ \lim\limits_{x \to 0} \frac{e^x-1-x}{\ln{(1+x)} - x}
= \frac{0}{0} 
= \lim\limits_{x \to 0} \frac{e^x-1}{\frac{1}{x+1} - 1}
= \lim\limits_{x \to 0} -\frac{e^x-1}{\frac{x}{x+1}}
= \frac{0}{0}
= $$

$$ = \lim\limits_{x \to 0} -\frac{e^x}{\frac{(1+x)-x}{(x+1)^2}}
= -1 $$

\endgroup
\end{document}