\documentclass{article}
\usepackage[utf8]{inputenc}
\usepackage{amsmath}
\usepackage{environ}
\usepackage[T2A,T1]{fontenc}
\usepackage[russian]{babel}
\usepackage[letterpaper,top=2cm,bottom=2cm,left=3cm,right=3cm,marginparwidth=1.75cm]{geometry}
\usepackage{xcolor}

\begin{document}
\textbf{â„– 7} 

$$ \int_{1}^{2} x\ln^2{x} dx 
= \begin{Vmatrix} \int f \,dg = fg - \int g \ df \end{Vmatrix} 
= \begin{Vmatrix} f = \ln^2{x} &  g = \frac{x^2}{2} \\
                 df = \frac{2\ln{x}}{x}dx  & dg = x dx \end{Vmatrix} 
= \ln^2{(x)} \cdot \frac{x^2}{2} - \int \frac{x^2}{2} \cdot \frac{2\ln{x}}{x} dx 
= $$

$$ = \ln^2{(x)} \cdot \frac{x^2}{2} - \int x\ln{x} dx 
= \begin{Vmatrix} f = \ln{x} &  g = \frac{x^2}{2} \\
                 df = \frac{1}{x}dx  & dg = x dx \end{Vmatrix} 
= \ln^2{(x)} \cdot \frac{x^2}{2} - \ln{(x)} \cdot \frac{x^2}{2} - \frac{1}{2} \int x dx
= $$

$$ = \left( \ln^2{(x)} \cdot \frac{x^2}{2} - \ln{(x)} \cdot \frac{x^2}{2} - \frac{1}{2} \cdot \frac{x^2}{2}  \right) \bigg\vert_{1}^{2}
= \left( 2\ln^2{2} - 2\ln{2} + 1 \right) - \left( 0 - 0 + \frac{1}{4} \right)
= 2\ln^2{2} - 2\ln{2} + \frac{3}{4} $$

\end{document}