\documentclass{article}
\usepackage[utf8]{inputenc}
\usepackage{amsmath}
\usepackage{environ}
\usepackage[T2A,T1]{fontenc}
\usepackage[russian]{babel}
\usepackage{hyperref}
\usepackage[letterpaper,top=2cm,bottom=2cm,left=3cm,right=3cm,marginparwidth=1.75cm]{geometry}

\begin{document}

\textbf{â„– 8} 

\begingroup
\Large

$$ \lim\limits_{x \to 0} \left( \frac{\sqrt{1+3x} - \sqrt[3]{1=5x}}{\sqrt[3]{1+3x} - \sqrt{1=5x}} \right)
= \frac{0}{0}
= $$

$$ = \lim\limits_{x \to 0} \left( \frac{\frac{3}{2\sqrt{1+3x}} - \frac{-5}{3(1-5x)^{\frac{2}{3}}}}{\frac{3}{3(1+3x)^{\frac{2}{3}}} - \frac{-5}{2 \sqrt{1-5x}}} \right)
= \frac{ \frac{3}{2} + \frac{5}{3} }{ 1  + \frac{5}{2} }
= \frac{19}{6} \cdot \frac{2}{7}
= \frac{19}{21}$$

\endgroup
\end{document}