\documentclass{article}
\usepackage[utf8]{inputenc}
\usepackage{amsmath}
\usepackage{environ}
\usepackage[T2A,T1]{fontenc}
\usepackage[russian]{babel}
\usepackage{hyperref}
\usepackage[letterpaper,top=2cm,bottom=2cm,left=3cm,right=3cm,marginparwidth=1.75cm]{geometry}


\begin{document}

\textbf{â„– 16} 

\begingroup
\Large

$$ \lim_{n\to \infty} \left( \frac{n-\frac{1}{n}}{n+\frac{1}{n}} \right)^{n}
= \lim_{n\to \infty} \left( \frac{n^2-1}{n^2+1} \right)^{n}
= 1^{\infty} 
= $$

$$ = e^{\lim\limits_{n\to\infty} \frac{\ln{\frac{n^2-1}{n^2+1}}}{\frac{1}{n}}}
= e^{\frac{0}{0}}
= e^{\lim\limits_{n\to\infty} \frac{\frac{n^2-1}{n^2+1} \frac{2n(n^2+1)-(n^2-1)2n}{(n^2+1)^2}}{-\frac{1}{n^2}}} 
= e^{\lim\limits_{n\to\infty} -\frac{4n}{(n^2-1)(n^2+1)}n^2}
= $$

$$ = e^{\lim\limits_{n\to\infty} -\frac{4n^3}{n^4-1}}
= e^{\lim\limits_{n\to\infty} -\frac{4n^3}{n^4(1-\frac{1}{n^4})}} 
= e^{0} 
= 1$$

\endgroup
\end{document}