\documentclass{article}
\usepackage[utf8]{inputenc}
\usepackage{amsmath}
\usepackage{environ}
\usepackage[T2A,T1]{fontenc}
\usepackage[russian]{babel}
\usepackage{hyperref}
\usepackage[letterpaper,top=2cm,bottom=2cm,left=3cm,right=3cm,marginparwidth=1.75cm]{geometry}

\begin{document}

\textbf{â„– 26} 

\begingroup
\Large

$$ \lim\limits_{x\to 2} \frac{f(x) - f(2)}{x^{\frac{1}{3}} - 2^{\frac{1}{3}}}
= \begin{vmatrix}
a^3 - b^3 = (a-b)(a^2 + ab + b^2)
\end{vmatrix}
= $$

$$ = \lim\limits_{x\to 2} \frac{(f(x) - f(2)) (x^{\frac{2}{3}} + 2^{\frac{1}{3}} x^{\frac{1}{3}} + 2^{\frac{2}{3}})} {(x^{\frac{1}{3}} - 2^{\frac{1}{3}}) (x^{\frac{2}{3}} + 2^{\frac{1}{3}} x^{\frac{1}{3}} + 2^{\frac{2}{3}})} 
= $$

$$ = \lim\limits_{x\to 2} \frac{(f(x) - f(2)) (x^{\frac{2}{3}} + 2^{\frac{1}{3}} x^{\frac{1}{3}} + 2^{\frac{2}{3}})} {x-2}
= \frac{0}{0}
= $$

$$ = \left( 2^{\frac{2}{3}} + 2^{\frac{2}{3}} + 2^{\frac{2}{3}} \right) f'(2)
= 3 \cdot 2^{\frac{2}{3}} \cdot f'(2)$$

\endgroup
\end{document}