\documentclass{article}
\usepackage[utf8]{inputenc}
\usepackage{amsmath}
\usepackage{environ}
\usepackage[T2A,T1]{fontenc}
\usepackage[russian]{babel}
\usepackage{hyperref}
\usepackage[letterpaper,top=2cm,bottom=2cm,left=3cm,right=3cm,marginparwidth=1.75cm]{geometry}


\begin{document}

\textbf{â„– 3} 

\begingroup
\Large

$$ \lim_{x\to +\infty} \left( \frac{2}{\pi} \arctg{x} \right)^{x}
= 1^{\infty} 
= e^{\lim\limits_{x\to +\infty} \ln{\left( \frac{2}{\pi} \arctg{x} \right)^{x}}}
= $$

$$ = e^{\lim\limits_{x\to +\infty} \frac{ \ln \left({\frac{2}{\pi}}\arctg{x} \right)}{\frac{1}{x}}}
=  
\begin{Vmatrix}
\lim\limits_{x\to +\infty} \arctg(x) = \frac{\pi}{2}
\end{Vmatrix}
= e^{\frac{0}{0}}
= e^{\lim\limits_{x\to +\infty} \frac{\left( \ln{\frac{2}{\pi}} + \ln{\arctg{x}} \right)}{\frac{1}{x}}} 
= $$

$$ = e^{\lim\limits_{x\to +\infty} \frac{\frac{1}{\arctg(x)} \frac{1}{1+x^2}}{-\frac{1}{x^2}}}
= e^{\lim\limits_{x\to +\infty} -\frac{x^2}{\arctg(x)(1+x^2)}}
= e^{\lim\limits_{x\to +\infty} -\frac{x^2}{x^2 \arctg(x)(1+\frac{1}{x^2})}}
= $$

$$ = e^{\lim\limits_{x\to +\infty} -\frac{1}{\arctg(x)(1+\frac{1}{x^2})}} 
= e^{-\frac{1}{\frac{\pi}{2}}}
= e^{-\frac{2}{\pi}} $$

\endgroup
\end{document}