\documentclass{article}
\usepackage[utf8]{inputenc}
\usepackage{amsmath}
\usepackage{environ}
\usepackage[T2A,T1]{fontenc}
\usepackage[russian]{babel}
\usepackage[letterpaper,top=2cm,bottom=2cm,left=3cm,right=3cm,marginparwidth=1.75cm]{geometry}

\begin{document}
\textbf{â„– 14} 

$$ \lim\limits_{x \to 0} \frac{\left( \sqrt{1 + x^2} + x \right)^{2018} - \left( \sqrt{1 + x^2} - x \right)^{2018})}{x} 
= \frac{0}{0}
=  $$

$$ = 2018\left( \sqrt{1 + x^2} + x \right)^{2017}\left( 1 + \frac{2x}{2\sqrt{1+x^2}} \right) - 2018\left( \sqrt{1 + x^2} - x \right)^{2017}\left( \frac{2x}{2\sqrt{1+x^2}} - 1 \right)
= $$

$$ = 2018 - 2018 \cdot (-1) 
= 2 \cdot 2018 $$

\end{document}