\documentclass{article}
\usepackage[utf8]{inputenc}
\usepackage{amsmath}
\usepackage{environ}
\usepackage[T2A,T1]{fontenc}
\usepackage[russian]{babel}
\usepackage[letterpaper,top=2cm,bottom=2cm,left=3cm,right=3cm,marginparwidth=1.75cm]{geometry}
\usepackage{xcolor}

\begin{document}
\textbf{№ 20} 
\\
\\ см. также {\color{blue}MAF} 2018-03-03 olympiad № 20
\\ см. также {\color{red}MAE} 2021-04-24 olympiad № 21
\\ см. также {\color{red}MAE} 2021-07-31 exam № 12

$$ \sum_{n=1}^{\infty} \frac{1}{9n^2+3n-2} $$

\begin{enumerate}

\item Transform the denominator

$$ D = (3)^2 + (-4)\times9\times(-2)=81=9^2 $$

$$ n_1 = \frac{-3+9}{18}=\frac{1}{3} $$
$$ n_2 = \frac{-3-9}{18}=-\frac{2}{3} $$

$$\sum_{n=1}^{\infty} \frac{1}{9n^2+3n-2} 
= \sum_{n=1}^{\infty} \frac{1}{9(n-\frac{1}{3})(n+\frac{2}{3})} 
= \sum_{n=1}^{\infty} \frac{1}{(3n-1)(3n+2)}$$

\item Divide the denominator

$$\frac{1}{(3n-1)(3n+2)} 
= \frac{A}{3n-1} + \frac{B}{3n+2} 
= \frac{A(3n+2)+B(3n-1)}{(3n-1)(3n+2)} 
= \frac{3An+2A+3Bn-B}{(3n-1)(3n+2)}$$

$$ 3An+2A+3Bn-B = 1 $$

$$
\left\{
  \begin{array}{ccc}
    3An + 3Bn = 0 \\
    2A-B = 1 \\
  \end{array}\Leftrightarrow
\right.
\left\{
  \begin{array}{ccc}
    A = -B \\
    -2B - B = 1 \\
  \end{array}\Leftrightarrow
\right.
\left\{
  \begin{array}{ccc}
    A = \frac{1}{3} \\
    B = -\frac{1}{3} \\
  \end{array}
\right.
$$

$$ \sum_{n=1}^{\infty} \frac{1}{(3n-1)(3n+2)} 
= \sum_{n=1}^{\infty} \left(\frac{1}{3(3n-1)} - \frac{1}{3(3n+2)}\right) $$

\item Find the sum of the series

$$ \sum_{n=1}^{\infty} \left(\frac{1}{3(3n-1)} - \frac{1}{3(3n+2)}\right) 
= S_n = a_1+a_2+...+a_{n-1}+a_n 
= $$

$$ = \frac{1}{6} - \underbrace{\frac{1}{15} + \frac{1}{15}}_{0} - \underbrace{\frac{1}{24} + \frac{1}{24}}_{0} - \frac{1}{33} + ..... - \frac{1}{3(3n+2)} 
= \frac{1}{6} - \frac{1}{3(3n+2)} $$

\item Find the limit
$$S = \lim_{n\to\infty} S_n 
= \lim_{n\to\infty} \left(\frac{1}{6} - \underbrace{\frac{1}{3(3n+2)}}_{0}\right) 
= \frac{1}{6} $$


\end{enumerate}
\end{document}